ironfleet/src/Dafny/Distributed/Services/Lock/Main.i.dfy
@@ -6,7 +6,7 @@ include "../../Impl/Lock/PacketParsing.i.dfy"
 include "../../Impl/Lock/UdpLock.i.dfy"
 include "../../Impl/Lock/Host.i.dfy"
 include "AbstractService.s.dfy"
-// include "../../Protocol/Lock/RefinementProof/Refinement.i.dfy"
+include "../../Protocol/Lock/RefinementProof/DistributedSystem.i.dfy"
 // include "../../Protocol/Lock/RefinementProof/RefinementProof.i.dfy"
 include "Marshall.i.dfy"
 
@@ -18,7 +18,7 @@ module Main_i refines Main_s {
     import opened UdpLock_i
     import opened Host_i
     import opened AS_s = AbstractServiceLock_s
-    // import opened Refinement_i
+    import opened DistributedSystem_i
     // import opened RefinementProof_i
     import opened MarshallProof_i
 
@@ -34,44 +34,185 @@ module Main_i refines Main_s {
         ensures  forall i :: 0 <= i < |db| ==> Service_Correspondence(db[i].environment.sentPackets, sb[i]);
         */
     {
-        var history := [config[0]];
-        sb := [ServiceState'(Collections__Maps2_s.mapdomain(db[0].servers), history)];
+        var lb := ImplToProtocol(config, db);
+        sb := ProtocolToSpec(config, lb);
+    }
 
-        // First prove Service_Init()
-        assert forall ep :: ep in config <==> ep in Collections__Maps2_s.mapdomain(db[0].servers);
-    
-        var i := 1;
-        while (i < |db|)
-            decreases |db| - i;
-            invariant 0 <= i <= |db|;
-            invariant |sb| == i;
-            invariant forall k :: 1 <= k < |sb| ==> sb[k].hosts == Collections__Maps2_s.mapdomain(db[k].servers);
 
-            // Invariants for proving initial state
-            invariant sb[0].history == [config[0]];
-            invariant config[0] in Collections__Maps2_s.mapdomain(db[0].servers);
-            invariant sb[0].hosts == Collections__Maps2_s.mapdomain(db[0].servers);
-        {
-            var impl_state := db[i];
-            var hosts := impl_state.servers.Keys;  // set of server endpoints
-            var host_states := impl_state.servers.Values;  // set of node HostStates
-            
-            // Find node holding the lock and add to history
-            var hs_set := host_states;
-            while ( hs_set != {} )
-                decreases hs_set;
+ 
+    /* Takes a sequence of impolementation states and returns a corresponding sequence of 
+    protocol states
+    */
+    lemma ImplToProtocol(config:ConcreteConfiguration, db:seq<DS_State>) returns (lb:seq<LS_State>) 
+        requires |config| > 0;
+        requires SeqIsUnique(config);
+        requires |db| > 0;
+        requires DS_Init(db[0], config);
+        requires forall i {:trigger DS_Next(db[i], db[i+1])} :: 0 <= i < |db| - 1 ==> DS_Next(db[i], db[i+1]);
+        ensures  |db| == |lb|; //
+        ensures  LS_Init(lb[0], config); //
+        ensures  forall i :: 0 <= i < |lb| - 1 ==>  LS_Next(lb[i], lb[i+1]);
+        // ensures  forall i :: 0 <= i < |db| ==> Service_Correspondence(db[i].environment.sentPackets, sb[i]);
+    {
+        // Construct LS_State.environment
+        var sentPackets := set p | p in db[0].environment.sentPackets :: LPacket(p.dst, p.src, AbstractifyCMessage(DemarshallData(p.msg)));
+        var hostInfo := convertHostInfo(db[0].environment.hostInfo);
+        var nextStep : LEnvStep<EndPoint, LockMessage>;
+        match db[0].environment.nextStep  {
+            case LEnvStepHostIos(actor, ios)    => 
             {
-                var hs :| hs in hs_set;
-                if (hs.node_impl.node.held) {
-                    history := history + [hs.node_impl.localAddr];
-                    break;
-                }
-                hs_set := hs_set - { hs };
+                var new_ios := convertLEnvStepHostIos(ios);
+                nextStep := LEnvStepHostIos(actor, new_ios);
             }
-            sb := sb + [ServiceState'(hosts, history)];
+            case LEnvStepDeliverPacket(p)       => 
+            {
+                var new_packet := LPacket(p.dst, p.src, AbstractifyCMessage(DemarshallData(p.msg)));
+                nextStep := LEnvStepDeliverPacket(new_packet);
+            }
+            case LEnvStepAdvanceTime            => 
+                nextStep := LEnvStepAdvanceTime();
+            case LEnvStepStutter                => 
+                nextStep := LEnvStepStutter();
+        }
+        var env := LEnvironment(db[0].environment.time,
+                                sentPackets,
+                                hostInfo,
+                                nextStep);
+
+        // Construct LS_State.servers
+        var servers :=   map s | s in db[0].servers :: db[0].servers[s].node;
+        lb := [LS_State(env, servers)];
+    }
+
+
+    /* Helper: Takes a seq<LIoOp<EndPoint, seq<byte>>> belonging to a ds state and returns
+    a corresponding seq<LIoOp<EndPoint, LockMessage>> belonging to an ls state 
+    */
+    lemma convertLEnvStepHostIos(s1: seq<LIoOp<EndPoint, seq<byte>>>) returns (s2: seq<LIoOp<EndPoint, LockMessage>>)
+        ensures |s1| == |s2|;
+        ensures forall i :: 0 <= i < |s1| ==> (
+            s1[i].LIoOpSend? ==> s2[i] == LIoOpSend(LPacket(s1[i].s.dst, s1[i].s.src, AbstractifyCMessage(DemarshallData(s1[i].s.msg))))
+        );
+        ensures forall i :: 0 <= i < |s1| ==> (
+            s1[i].LIoOpReceive? ==> s2[i] == LIoOpReceive(LPacket(s1[i].r.dst, s1[i].r.src, AbstractifyCMessage(DemarshallData(s1[i].r.msg))))
+        );
+        ensures forall i :: 0 <= i < |s1| ==> (
+            s1[i].LIoOpTimeoutReceive? ==> s2[i] == LIoOpTimeoutReceive()
+        );
+        ensures forall i :: 0 <= i < |s1| ==> (
+            s1[i].LIoOpReadClock? ==> s2[i] == LIoOpReadClock(s1[i].t)
+        );
+    {
+        s2 := [];
+        var i := 0;
+        while (i < |s1|)
+            decreases |s1| - i;
+            invariant 0 <= i <= |s1|;
+            invariant i == |s2|;
+            invariant forall k :: 0 <= k < i ==> (
+                s1[k].LIoOpSend? ==> s2[k] == LIoOpSend(LPacket(s1[k].s.dst, s1[k].s.src, AbstractifyCMessage(DemarshallData(s1[k].s.msg))))
+            );
+            invariant forall k :: 0 <= k < i ==> (
+                s1[k].LIoOpReceive? ==> s2[k] == LIoOpReceive(LPacket(s1[k].r.dst, s1[k].r.src, AbstractifyCMessage(DemarshallData(s1[k].r.msg))))
+            );
+            invariant forall k :: 0 <= k < i ==> (
+                s1[k].LIoOpTimeoutReceive? ==> s2[k] == LIoOpTimeoutReceive()
+            );
+            invariant forall k :: 0 <= k < i ==> (
+                s1[k].LIoOpReadClock? ==> s2[k] == LIoOpReadClock(s1[k].t)
+            );
+        {
+            match s1[i] {
+                case LIoOpSend(s)               =>
+                {
+                    s2 := s2 + [LIoOpSend(LPacket(s.dst, s.src, AbstractifyCMessage(DemarshallData(s.msg))))];
+                }
+                case LIoOpReceive(r)            =>
+                {
+                    s2 := s2 + [LIoOpReceive(LPacket(r.dst, r.src, AbstractifyCMessage(DemarshallData(r.msg))))];
+                }
+                case LIoOpTimeoutReceive()      =>
+                {
+                    s2 := s2 + [LIoOpTimeoutReceive()];
+                }
+                case LIoOpReadClock(t)          =>
+                {
+                    s2 := s2 + [LIoOpReadClock(t)];
+                }
+            }
             i := i + 1;
         }
-        assert i == |db|;
-        assert i == |sb|;
+    }
+
+
+
+    /* Helper: Takes a seq<LPacket<EndPoint, seq<byte>>> belonging to a ds state and 
+    returns a corresponding seq<LPacket<EndPoint, LockMessage>> belonging 
+    to a ls state */
+    lemma byteSeqToLockMessageSeq(byte_seq:seq<LPacket<EndPoint, seq<byte>>>) returns (lock_msg_seq:seq<LPacket<EndPoint, LockMessage>>)
+        ensures |byte_seq| == |lock_msg_seq|;
+        ensures forall i :: 0 <= i < |byte_seq| ==> byte_seq[i].dst == lock_msg_seq[i].dst;
+        ensures forall i :: 0 <= i < |byte_seq| ==> byte_seq[i].src == lock_msg_seq[i].src;
+        ensures forall i :: 0 <= i < |byte_seq| ==> AbstractifyCMessage(DemarshallData(byte_seq[i].msg)) == lock_msg_seq[i].msg;
+    {
+        lock_msg_seq := [];
+        var i := 0;
+        while (i < |byte_seq|) 
+            decreases |byte_seq| - i;
+            invariant 0 <= i <= |byte_seq|;
+            invariant |lock_msg_seq| == i;
+            invariant forall k :: 0 <= k < i ==> byte_seq[k].dst == lock_msg_seq[k].dst;
+            invariant forall k :: 0 <= k < i ==> byte_seq[k].src == lock_msg_seq[k].src;
+            invariant forall k :: 0 <= k < i ==> AbstractifyCMessage(DemarshallData(byte_seq[k].msg)) == lock_msg_seq[k].msg;
+        {
+            var next_packet := LPacket(byte_seq[i].dst, byte_seq[i].src, AbstractifyCMessage(DemarshallData(byte_seq[i].msg)));
+            lock_msg_seq := lock_msg_seq + [next_packet];
+            i := i+1;
+        }
+        assert i == |lock_msg_seq| == |byte_seq|;
+    }
+
+    /* Helper: Takes a hostInfo:map<EndPoint, LHostInfo<EndPoint, seq<byte>>> belonging 
+    to a ds state and returns a corresponding hostInfo:map<EndPoint, LHostInfo<EndPoint, LockMessage>> 
+    belonging to a ls state */
+    lemma convertHostInfo(h1: map<EndPoint, LHostInfo<EndPoint, seq<byte>>>) returns (h2: map<EndPoint, LHostInfo<EndPoint, LockMessage>>) 
+        ensures |h1| == |h2|; 
+        ensures forall ep :: ep in h1 ==> ep in h2;
+        ensures forall ep :: ep in h1 ==> |h1[ep].queue| == |h2[ep].queue|; 
+        ensures forall ep :: ep in h1 ==> (forall i :: 0 <= i < |h1[ep].queue| ==> h1[ep].queue[i].dst == h2[ep].queue[i].dst);
+        ensures forall ep :: ep in h1 ==> (forall i :: 0 <= i < |h1[ep].queue| ==> h1[ep].queue[i].src == h2[ep].queue[i].src);
+        ensures forall ep :: ep in h1 ==> (forall i :: 0 <= i < |h1[ep].queue| ==> AbstractifyCMessage(DemarshallData(h1[ep].queue[i].msg)) == h2[ep].queue[i].msg);
+    {
+        h2 := map[];
+        var keys := h1.Keys;
+        while keys != {}
+            decreases keys
+            invariant h2.Keys <= h1.Keys;
+            invariant keys + h2.Keys == h1.Keys;
+            invariant |keys| + |h2| == |h1|;
+            invariant forall ep :: ep in h1 && !(ep in keys) ==> ep in h2;
+            invariant forall ep :: ep in h2 ==> |h1[ep].queue| == |h2[ep].queue|;
+            invariant forall ep :: ep in h2 ==> (forall i :: 0 <= i < |h2[ep].queue| ==> h1[ep].queue[i].dst == h2[ep].queue[i].dst); 
+            invariant forall ep :: ep in h2 ==> (forall i :: 0 <= i < |h2[ep].queue| ==> h1[ep].queue[i].src == h2[ep].queue[i].src); 
+            invariant forall ep :: ep in h2 ==> (forall i :: 0 <= i < |h2[ep].queue| ==> AbstractifyCMessage(DemarshallData(h1[ep].queue[i].msg)) == h2[ep].queue[i].msg); 
+        {
+            var k :| k in keys;
+            var lock_msg_queue := byteSeqToLockMessageSeq(h1[k].queue);
+            h2 := h2[k := LHostInfo(lock_msg_queue)];
+            keys := keys - {k};
+        }
+    }
+
+
+    lemma ProtocolToSpec(config:ConcreteConfiguration, lb:seq<LS_State>) returns (sb:seq<ServiceState>)
+        // requires |lb| > 0;
+        // requires LS_Init(lb[0], config);
+        // requires forall i :: 0 <= i < |lb| - 1 ==>  LS_Next(lb[i], lb[i+1]);
+        // ensures  |lb| == |sb|;
+        // ensures  Service_Init(sb[0], Collections__Maps2_s.mapdomain(lb[0].servers));
+        // ensures  forall i {:trigger Service_Next(sb[i], sb[i+1])} :: 0 <= i < |sb| - 1 ==> sb[i] == sb[i+1] || Service_Next(sb[i], sb[i+1]);
+        // ensures  forall i :: 0 <= i < |db| ==> Service_Correspondence(db[i].environment.sentPackets, sb[i]);
+    {
+
     }
 }
